Refactored TrichDec, with a much better automation.

Structures/TrichDec.v
@@ -1,99 +1,91 @@
 Require Export RCCBase.
 
-Require Export LinDec.
-
 Set Implicit Arguments.
-
-Hint Constructors comparison : core.
 
 Class TrichDec : Type :=
 {
     carrier : Type;
     trich_lt : carrier -> carrier -> Prop;
     trich_lt_antisym :
-      forall x y : carrier, trich_lt x y -> ~ trich_lt y x;
+      forall {x y : carrier}, trich_lt x y -> ~ trich_lt y x;
     trich_lt_trans :
-      forall x y z : carrier, trich_lt x y -> trich_lt y z -> trich_lt x z;
-    trichb : carrier -> carrier -> comparison;
-    trichb_spec :
-      forall x y : carrier, CompareSpec (x = y) (trich_lt x y) (trich_lt y x) (trichb x y);
+      forall {x y z : carrier}, trich_lt x y -> trich_lt y z -> trich_lt x z;
+    cmp : carrier -> carrier -> comparison;
+    cmp_spec :
+      forall x y : carrier, CompareSpec (x = y) (trich_lt x y) (trich_lt y x) (cmp x y);
 }.
 
-Infix "<" := trich_lt (at level 70).
-Infix "<?>" := trichb (at level 70).
+Coercion carrier : TrichDec >-> Sortclass.
 
-Hint Resolve trich_lt_antisym trich_lt_trans : core.
+(* Hint Resolve trich_lt_trans : core. *)
 
-Definition TrichDec_ltb {A : TrichDec} (x y : @carrier A) : bool :=
-match x <?> y with
+Definition trich_ltb {A : TrichDec} (x y : A) : bool :=
+match cmp x y with
     | Lt => true
     | _ => false
 end.
 
-Notation "x <? y" := (TrichDec_ltb x y) (at level 70).
+Definition trich_leb {A : TrichDec} (x y : A) : bool :=
+match cmp x y with
+    | Lt | Eq => true
+    | Gt      => false
+end.
+
+Definition trich_eqb {A : TrichDec} (x y : A) : bool :=
+match cmp x y with
+    | Eq => true
+    | _  => false
+end.
+
+Definition trich_le {A : TrichDec} (x y : A) : Prop :=
+  trich_lt x y \/ x = y.
+
+Infix "<?>" := cmp (at level 30).
+Infix "<?" := trich_ltb (at level 70).
+Notation "x >? y" := (trich_ltb y x) (at level 30).
+Infix "≤?" := trich_leb (at level 30).
+Notation "x >=? y" := (trich_leb y x) (at level 30).
+Infix "==?" := trich_eqb (at level 30).
+
+Infix "<" := trich_lt (at level 70).
+Notation "x > y" := (trich_lt y x) (at level 70, only parsing).
+(* Infix "≤" := trich_le (at level 30). *)
+Notation "x >= y" := (trich_le y x) (at level 70, only parsing).
 
 Lemma trich_lt_irrefl :
-  forall (A : TrichDec) (x : carrier),
+  forall {A : TrichDec} {x : A},
     ~ trich_lt x x.
 Proof.
   intros A x H. eapply trich_lt_antisym; eassumption.
 Qed.
 
-(* Hint Extern 0 =>
-match goal with
-    | H : _ < _ |- _ => apply trich_lt_irrefl in H; contradiction
-end
-  : core.
- *)
-Lemma trich_lt_antisym' :
-  forall (A : TrichDec) (x y : carrier),
-    trich_lt x y -> ~ trich_lt y x.
+Lemma trich_lt_connected :
+  forall {A : TrichDec} {x y : A},
+    ~ trich_lt x y -> ~ trich_lt y x -> x = y.
 Proof.
-  intros A x y.
-  intros Hxy Hyx.
-  eapply trich_lt_irrefl, trich_lt_trans; eassumption.
+  intros. destruct (cmp_spec x y).
+    assumption.
+    contradiction.
+    contradiction.
 Qed.
 
 Lemma trich_lt_comparison :
-  forall (A : TrichDec) (x y z : carrier),
-    trich_lt x z -> trich_lt x y \/ trich_lt y z.
+  forall {A : TrichDec} {x z : A},
+    trich_lt x z -> forall y : A, trich_lt x y \/ trich_lt y z.
 Proof.
-  intros. destruct (trichb_spec x y).
+  intros. destruct (cmp_spec x y).
     subst. auto.
     auto.
     right. eapply trich_lt_trans; eassumption.
 Qed.
 
-Lemma trich_lt_trans' :
-  forall (A : TrichDec) (x y z : carrier),
-    trich_lt x y -> trich_lt y z -> trich_lt x z.
-Proof.
-  intros A x y z Hxy Hyz.
-  destruct (trichb_spec x z).
-    subst. contradict Hyz. apply trich_lt_antisym. assumption.
-    assumption.
-    destruct (trich_lt_comparison _ _ z y Hxy).
-      assumption.
-      contradict H0. apply trich_lt_antisym. assumption.
-Qed.
+(** comparison properties *)
 
-Lemma trich_lt_connected :
-  forall (A : TrichDec) (x y : carrier),
-    ~ trich_lt x y -> ~ trich_lt y x -> x = y.
+Lemma cmp_spec1 :
+  forall {A : TrichDec} (x y : A),
+    cmp x y = Lt <-> trich_lt x y.
 Proof.
-  intros. destruct (trichb_spec x y).
-    assumption.
-    contradiction.
-    contradiction.
-Qed.
-
-Hint Resolve trich_lt_irrefl trich_lt_comparison trich_lt_trans trich_lt_connected : core.
-
-Lemma trichb_spec1 :
-  forall (A : TrichDec) (x y : carrier),
-    trichb x y = Lt <-> trich_lt x y.
-Proof.
-  intros. destruct (trichb_spec x y).
+  intros. destruct (cmp_spec x y).
     subst. split.
       inv 1.
       intro. contradict H. apply trich_lt_irrefl.
@@ -103,78 +95,198 @@ Proof.
       intro. contradict H. apply trich_lt_antisym. assumption.
 Qed.
 
-Lemma trichb_spec2 :
-  forall (A : TrichDec) (x y : carrier),
-    trichb x y = Eq <-> x = y.
+Lemma cmp_spec2 :
+  forall {A : TrichDec} (x y : A),
+    cmp x y = Eq <-> x = y.
 Proof.
-  intros. destruct (trichb_spec x y).
+  intros. destruct (cmp_spec x y).
     firstorder.
     split; inv 1. contradict H. apply trich_lt_irrefl.
     split; inv 1. contradict H. apply trich_lt_irrefl.
 Qed.
 
-Lemma trichb_spec3 :
-  forall (A : TrichDec) (x y : carrier),
-    trichb x y = Gt <-> trich_lt y x.
+Lemma cmp_spec3 :
+  forall {A : TrichDec} (x y : A),
+    cmp x y = Gt <-> trich_lt y x.
 Proof.
-  intros. destruct (trichb_spec x y);
+  intros. destruct (cmp_spec x y);
   firstorder; try congruence.
     contradict H0. subst. apply trich_lt_irrefl.
     contradict H0. apply trich_lt_antisym. assumption.
 Qed.
 
-Lemma trich_lt_trich :
-  forall (A : TrichDec) (x y : carrier),
-    trich_lt x y \/ x = y \/ trich_lt y x.
+Lemma CompOpp_cmp :
+  forall {A : TrichDec} {x y : A},
+    CompOpp (x <?> y) = (y <?> x).
 Proof.
-  intros. destruct (trichb_spec x y); auto.
+  intros.
+  destruct (cmp_spec x y), (cmp_spec y x);
+  cbn; subst; try reflexivity;
+  match goal with
+      | H : ?x < ?y |- _ =>
+          pose (trich_lt_antisym H); contradiction
+  end.
 Qed.
 
-Hint Resolve trichb_spec1 trichb_spec2 trichb_spec3 trich_lt_trich : core.
+Lemma cmp_refl :
+  forall {A : TrichDec} (x : A),
+    x <?> x = Eq.
+Proof.
+  intros.
+  destruct (cmp_spec x x).
+    reflexivity.
+    apply trich_lt_irrefl in H. contradiction.
+    apply trich_lt_irrefl in H. contradiction.
+Qed.
 
-Ltac trich := cbn; unfold TrichDec_ltb; repeat
-match goal with
-    | H : context [match ?x <?> ?y with | _ => _ end] |- _ =>
-        case_eq (x <?> y); intro
-    | |- context [match ?x <?> ?y with | _ => _ end] =>
-        case_eq (x <?> y); intro
-    | H : _ <?> _ = _ |- _ =>
-        rewrite ?trichb_spec1, ?trichb_spec2, ?trichb_spec3 in H
+Lemma trich_ltb_irrefl :
+  forall {A : TrichDec} (x : A),
+    x <? x = false.
+Proof.
+  intros.
+  unfold trich_ltb.
+  rewrite cmp_refl.
+  reflexivity.
+Qed.
+
+Lemma negb_trich_ltb :
+  forall {A : TrichDec} (x y : A),
+    negb (x <? y) = x >=? y.
+Proof.
+  intros.
+  unfold trich_ltb, trich_leb.
+  destruct (cmp_spec x y), (cmp_spec y x);
+  cbn; subst; try reflexivity;
+  match goal with
+      | H : _ < _ |- _ => pose (trich_lt_antisym H); contradiction
+  end.
+Qed.
+
+Lemma trich_leb_refl :
+  forall {A : TrichDec} (x : A),
+    x ≤? x = true.
+Proof.
+  intros.
+  unfold trich_leb.
+  rewrite cmp_refl.
+  reflexivity.
+Qed.
+
+Lemma negb_trich_leb :
+  forall {A : TrichDec} (x y : A),
+    negb (x ≤? y) = x >? y.
+Proof.
+  intros.
+  unfold trich_ltb, trich_leb.
+  destruct (cmp_spec x y), (cmp_spec y x);
+  cbn; subst; try reflexivity;
+  match goal with
+      | H : _ < _ |- _ => pose (trich_lt_antisym H); contradiction
+  end.
+Qed.
+
+Lemma trich_eqb_refl :
+  forall {A : TrichDec} (x : A),
+    x ==? x = true.
+Proof.
+  intros.
+  unfold trich_eqb.
+  rewrite cmp_refl.
+  reflexivity.
+Qed.
+
+(* Newest lemmas *)
+
+Lemma trichb_Gt_to_Lt :
+  forall {A : TrichDec} {x y : A},
+    x <?> y = Gt -> y <?> x = Lt.
+Proof.
+  intros A x y Hxy.
+  rewrite ?cmp_spec1, <- ?cmp_spec3 in *.
+  assumption.
+Qed.
+
+Lemma trichb_trans_Lt :
+  forall {A : TrichDec} {x y z : A},
+    x <?> y = Lt -> y <?> z = Lt -> x <?> z = Lt.
+Proof.
+  intros A x y z Hxy Hyz.
+  rewrite cmp_spec1 in *.
+  eapply trich_lt_trans; eassumption.
+Qed.
+
+Ltac trich :=
+  cbn;
+  unfold trich_ltb, trich_leb, trich_eqb;
+repeat match goal with
+(* General contradictions *)
+    | H : False |- _ => contradiction
+    | H : ?x <> ?x |- _ => contradiction H; reflexivity
+(* Easy contradictions from TrichDec properties *)
+    | H : ?x < ?x |- _ => apply trich_lt_irrefl in H; contradiction
     | H : ?x < ?y, H' : ?y < ?x |- _ =>
         pose (trich_lt_antisym x y H); contradiction
-end; dec; cbn; subst; try
-match goal with
-    | H : ?x <> ?x |- _ => contradiction H; reflexivity
-    | H : ?x < ?x |- _ => apply trich_lt_irrefl in H; contradiction
-end; dec.
+(* Deduce equality and substitute *)
+    | H : _ <?> _ = Eq |- _ => rewrite cmp_spec2 in H; subst
+    | H : ~ ?x < ?y, H' : ~ ?y < ?x |- _ =>
+        pose (trich_lt_connected H H'); subst; clear H H'
+(* Computational properties of cmp *)
+    | H : context [?x <?> ?x] |- _ =>
+        rewrite cmp_refl in H
+    | |- context [?x <?> ?x] =>
+        rewrite cmp_refl
+    | H : context [CompOpp (_ <?> _)] |- _ =>
+        rewrite CompOpp_cmp in H
+    | |- context [CompOpp (_ <?> _)] =>
+        rewrite CompOpp_cmp
+(* Computational properties of derived operations *)
+    | H : context [?x <? ?x] |- _ =>
+        rewrite trich_ltb_irrefl in H
+    | |- context [?x <? ?x] =>
+        rewrite trich_ltb_irrefl
+    | H : context [?x ≤? ?x] |- _ =>
+        rewrite trich_leb_refl in H
+    | |- context [?x ≤? ?x] =>
+        rewrite trich_leb_refl
+    | H : context [?x ==? ?x] |- _ =>
+        rewrite trich_eqb_refl in H
+    | |- context [?x ==? ?x] =>
+        rewrite trich_eqb_refl
+(* Transitivity *)
+    | Hxy : ?x < ?y, Hyz : ?y < ?z |- _ =>
+        assert (x < z) by (eapply trich_lt_trans; eauto)
+    | Hxy : _ <?> _ = Gt |- _ => apply trichb_Gt_to_Lt in Hxy
+    | Hxy : ?x <?> ?y = Lt, Hyz : ?y <?> ?z = Lt |- _ =>
+        match goal with
+            | Hyz : x <?> z = Lt |- _ => idtac
+            | _ => pose (Hxz := trichb_trans_Lt Hxy Hyz); clearbody Hxz
+        end
+(* Case analysis *)
+    | H : context [match ?x <?> ?y with | _ => _ end] |- _ =>
+        destruct (cmp_spec x y)
+    | |- context [match ?x <?> ?y with | _ => _ end] =>
+        destruct (cmp_spec x y)
+(* reverse cases *)
+(*     | H : _ <?> _ = _ |- _ =>
+        rewrite ?cmp_spec1, ?cmp_spec3 in H
+ *)    | _ => subst; auto; try congruence
+end;
+  subst; auto; try congruence.
 
-#[refine]
-Instance TrichDec_to_LinDec (A : TrichDec) : LinDec :=
-{
-    carrier := @carrier A;
-    leq x y := ~ trich_lt y x;
-    leqb x y :=
-      match trichb x y with
-          | Gt => false
-          | _ => true
-      end
-}.
-Proof.
-  apply trich_lt_irrefl.
-  intros. apply trich_lt_connected; assumption.
-  intros; intro. decompose [or] (trich_lt_trich A z y); trich.
-  intros. decompose [or] (trich_lt_trich A x y); trich.
-  intros. case_eq (trichb x y); intro; trich.
-Defined.
+Ltac trich_aggresive :=
+repeat match goal with
+    | H : context [?x <?> ?y] |- _ => destruct (cmp_spec x y); subst
+    | |- context [?x <?> ?y] => destruct (cmp_spec x y); subst
+end.
 
-Coercion TrichDec_to_LinDec : TrichDec >-> LinDec.
+Ltac trich' := trich; try (trich_aggresive; trich; fail).
 
-Fixpoint trichb_nat (n m : nat) : comparison :=
+Fixpoint cmp_nat (n m : nat) : comparison :=
 match n, m with
     | 0, 0 => Eq
     | 0, _ => Lt
     | _, 0 => Gt
-    | S n', S m' => trichb_nat n' m'
+    | S n', S m' => cmp_nat n' m'
 end.
 
 #[refine]
@@ -182,7 +294,7 @@ Instance natlt : TrichDec :=
 {
     carrier := nat;
     trich_lt := Peano.lt;
-    trichb := trichb_nat
+    cmp := cmp_nat
 }.
 Proof.
   1-2: intros; lia.
@@ -190,29 +302,3 @@ Proof.
     1-3: constructor; lia.
     destruct (IHx' y'); constructor; lia.
 Defined.
-
-Lemma trichb_refl :
-  forall (A : TrichDec) (x : A),
-    x <?> x = Eq.
-Proof.
-  intros. rewrite trichb_spec2. trivial.
-Qed.
-
-Definition flipcomparison (o : comparison) : comparison :=
-match o with
-    | Lt => Gt
-    | Eq => Eq
-    | Gt => Lt
-end.
-
-Lemma trichb_flipcomparison :
-  forall (A : TrichDec) (x y : @carrier A), flipcomparison (x <?> y) = (y <?> x).
-Proof.
-  intros. destruct (trichb_spec y x), (trichb_spec x y); cbn; trich.
-Qed.
-
-Lemma ltb_negb_leqb :
-  forall (A : TrichDec) (x y : A), x <? y = negb (y <=? x).
-Proof.
-  intros. trich.
-Qed.
